theories/translation_map.v
@@ -1,0 +1,92 @@
+From Coq Require Import ssreflect.
+From stdpp Require Import strings gmap.
+From melocoton Require Import commons.
+
+Section TranslationMap.
+
+Context (A B : Type).
+Context `{Countable A}.
+Context `{Countable B}.
+Context `{Infinite A}.
+Context `{Infinite B}.
+
+Definition translation_map := gmap A B.
+
+Definition is_translation_map (m : translation_map) (MA : gset A) (MB : gset B) :=
+     gmap_inj m
+  /\ (forall k, k ∈ MA → k ∈ dom m)
+  /\ (forall k, k ∈ MB → (exists x, m !! x = Some k)).
+
+Lemma tm_insert_l m l MA MB : is_translation_map m MA MB ->
+  exists m', m ⊆ m' ∧ is_translation_map m' (MA ∪ {[l]}) MB.
+Proof.
+  intros HH.
+  destruct (m !! l) eqn:Heq.
+  + exists m. split; first done.
+    destruct HH as (HH1 & HH2 & HH3); split; first done.
+    split; last done.
+    intros k [Hin| -> % elem_of_singleton]%elem_of_union. 1: by apply HH2.
+    eapply elem_of_dom. by exists b.
+  + pose (fresh (map_to_set (fun a b => b) m : gset B)) as r.
+    exists (<[ l := r ]> m). destruct HH as (HH1 & HH2 & HH3). repeat split.
+    * by apply insert_subseteq.
+    * intros k1 k2 v. intros [[? ?]|[Hne1 Hk1]]%lookup_insert_Some [[? ?]|[Hne2 Hk2]]%lookup_insert_Some; subst.
+      - done.
+      - exfalso. eapply (is_fresh (map_to_set (fun a b => b) m : gset B)).
+        eapply elem_of_map_to_set. do 2 eexists; repeat split; try done.
+      - exfalso. eapply (is_fresh (map_to_set (fun a b => b) m : gset B)).
+        eapply elem_of_map_to_set. do 2 eexists; repeat split; try done.
+      - eapply HH1; done.
+    * intros k [Hin| -> % elem_of_singleton]%elem_of_union; rewrite dom_insert_L.
+      - eapply elem_of_union_r. eapply HH2. done.
+      - eapply elem_of_union_l, elem_of_singleton. done.
+    * intros k Hk. destruct (HH3 k Hk) as (x & Hx). exists x. rewrite lookup_insert_ne; first done.
+      intros <-. rewrite Heq in Hx. done.
+Qed.
+
+Lemma tm_insert_r m r MA MB : is_translation_map m MA MB ->
+  exists m', m ⊆ m' ∧ is_translation_map m' (MA) (MB ∪ {[r]}).
+Proof.
+  intros HH.
+  pose ((map_to_set (fun a b => b) m : gset B)) as mdom.
+  destruct (decide (r ∈ mdom)) as [Hin|Hnot].
+  + exists m. split; first done.
+    destruct HH as (HH1 & HH2 & HH3); split; first done.
+    split; first done.
+    intros k [Hink| -> % elem_of_singleton]%elem_of_union. 1: by apply HH3.
+    eapply elem_of_map_to_set in Hin. destruct Hin as (i & x & HS & ->).
+    exists i; done.
+  + pose (fresh (dom m)) as l.
+    exists (<[ l := r ]> m). destruct HH as (HH1 & HH2 & HH3). repeat split.
+    * apply insert_subseteq. eapply not_elem_of_dom. eapply is_fresh.
+    * intros k1 k2 v. intros [[? ?]|[Hne1 Hk1]]%lookup_insert_Some [[? ?]|[Hne2 Hk2]]%lookup_insert_Some; subst.
+      - done.
+      - exfalso. apply Hnot.
+        eapply elem_of_map_to_set. do 2 eexists; repeat split; try done.
+      - exfalso. apply Hnot.
+        eapply elem_of_map_to_set. do 2 eexists; repeat split; try done.
+      - eapply HH1; done.
+    * intros k Hk. rewrite dom_insert_L. eapply elem_of_union_r. by apply HH2.
+    * intros k [Hin| -> % elem_of_singleton]%elem_of_union.
+      - destruct (HH3 k Hin) as (v & Hv). exists v. rewrite lookup_insert_ne; first done. intros <-.
+        eapply (is_fresh (dom m)). eapply elem_of_dom. exists k. apply Hv.
+      - exists l. rewrite lookup_insert. done.
+Qed.
+
+Lemma tm_bulk_update (m:translation_map) (MA MA' : gset A) (MB MB' : gset B) :
+    is_translation_map m MA MB
+ -> MA ⊆ MA'
+ -> MB ⊆ MB'
+ -> exists (m':translation_map), m ⊆ m' /\ is_translation_map m' MA' MB'.
+Proof.
+  intros Hmap H3 H4.
+Abort.
+
+
+
+
+
+
+
+
+End TranslationMap.
